src/simple-proof/proof/CanonicalForms.v
@@ -62,9 +62,9 @@ Qed.
     [v = lambda(T')t]              #<br>#
     [G ⊢ T <: T']                   #<br>#
     [forall fresh y, G, y: T ⊢ t^y: U^y] *)
-Lemma val_typ_all_to_lambda: forall G v t T U,
+Lemma val_typ_all_to_lambda: forall G v x t T U,
     inert G ->
-    trm_val v t ->
+    trm_val x v t ->
     G ⊢ t : typ_all T U ->
     (exists L T' t',
         v = val_fun T' t' /\
@@ -73,14 +73,14 @@ Lemma val_typ_all_to_lambda: forall G v t T U,
 Proof.
   introv Hin Htv Ht.
   lets Htt: (general_to_tight_typing Hin Ht).
-  lets Hinv: (tight_to_invertible_v Hin Htv Htt).
+  lets Hinv: (tight_to_invertible_forall Hin Htv Htt).
   destruct (invertible_val_to_precise_lambda Hin Hinv) as [L [T' [U' [Htp [Hs1 Hs2]]]]].
   inversions Htp.
   exists (L0 \u L \u (dom G)) T' t0. repeat split~.
   intros. assert (HL: y \notin L) by auto. assert (HL0: y \notin L0) by auto.
   specialize (Hs2 y HL).
-  specialize (H2 y HL0).
-  eapply ty_sub; eauto. eapply narrow_typing in H2; eauto.
+  specialize (H3 y HL0).
+  eapply ty_sub; eauto. eapply narrow_typing in H3; eauto.
 Qed.
 
 (** * Objects under Inert Contexts *)
@@ -122,38 +122,39 @@ Qed.
     [G ⊢ t: U] *)
 Lemma val_mu_to_new: forall G v t T U a x,
     inert G ->
-    trm_val v t ->
+    x # G ->
+    trm_val x v t ->
     G ⊢ t: typ_bnd T ->
     G ⊢ trm_var (avar_f x) : open_typ x T ->
     record_has (open_typ x T) (dec_trm a U) ->
     exists t' ds,
       v = val_obj T ds /\
-      defs_has (open_defs x ds) (def_trm a t') /\
+      defs_has ds (def_trm a t') /\
       G ⊢ t': U.
 Proof.
-  introv Hi Htv Ht Hx Hr.
+  introv Hi HxG Htv Ht Hx Hr.
   lets Htt: (general_to_tight_typing Hi Ht).
-  lets Hinv: (tight_to_invertible_v Hi Htv Htt).
+  lets Hinv: (tight_to_invertible_v Hi HxG Htv Htt).
   inversions Hinv. inversions H.
   pick_fresh z. assert (z \notin L) as Hz by auto.
-  specialize (H3 z Hz).
+  specialize (H1 z Hz).
   assert (G /- open_defs x ds :: open_typ x T) as Hds by apply* renaming_def.
   destruct (record_has_ty_defs Hds Hr) as [d [Hh Hd]]. inversions Hd.
-  exists t0 ds. split*.
+  exists t0 (open_defs x ds). split*.
 Qed.
 
 Lemma strong_mu_to_new: forall G s x T,
     inert G ->
     ty_val_s G s x ->
     binds x (typ_bnd T) G ->
-    exists ds, binds x (val_obj T ds) s /\
+    exists ds, binds x (val_obj T (open_defs x ds)) s /\
                G /- open_defs x ds :: open_typ x T.
 Proof.
   introv Hi Hts Bi.
   inversions Hts.
   - pose proof (binds_func Bi H); subst T0; clear H.
     pose proof (general_to_tight_typing Hi H1).
-    pose proof (tight_to_invertible_v Hi (trm_val_fun _ _) H).
+    pose proof (tight_to_invertible_fun Hi (trm_val_fun x _ _) H).
     inversions H2. inversions H3.
   - pose proof (binds_func Bi H). inversions H1.
     exists ds; split; auto.
@@ -180,7 +181,7 @@ Proof.
   pose proof (corresponding_types Hst BiG).
   inversions H.
   - pose proof (binds_func BiG H0). subst T0.
-    destruct (val_typ_all_to_lambda Hin (trm_val_fun _ _) H2)
+    destruct (val_typ_all_to_lambda Hin (trm_val_fun x _ _) H2)
       as [L' [S' [t' [Heq [Hs1' Hs2']]]]].
     exists (L \u L' \u (dom G)) S' t'. inversions Heq.
     repeat_split_right; eauto.
@@ -208,7 +209,7 @@ Lemma canonical_forms_obj: forall G s x a T,
   inert G ->
   strongly_typed G s ->
   G ⊢ trm_var (avar_f x) : (typ_rcd (dec_trm a T)) ->
-  (exists S ds t, binds x (val_obj S ds) s /\
+  (exists S ds t, binds x (val_obj S (open_defs x ds)) s /\
                   defs_has (open_defs x ds) (def_trm a t) /\
                   G ⊢ t : T).
 Proof.
